systems/Sorting.v
@@ -1,0 +1,87 @@
+Require Import List.
+Import ListNotations.
+Require Import Sorting.Permutation.
+
+Section Sorting.
+  Variable t : Type.
+  Variable le : t -> t -> bool.
+
+  Variable le_reflexive :
+    forall x, le x x = true.
+
+  Variable le_transitive :
+    forall x y z,
+      le x y = true ->
+      le y z = true ->
+      le x z = true.
+
+  Variable le_total :
+    forall x y,
+      le x y = true \/ le y x = true.
+
+  Inductive sorted : list t -> Prop :=
+  | SortedNil :
+      sorted []
+  | SortedSingleton :
+      forall x, sorted [x]
+  | SortedCons :
+      forall x y l,
+        sorted (y :: l) ->
+        le x y = true ->
+        sorted (x :: y :: l).
+
+  (* from Coq stdlib mergesort implementation *)
+  Fixpoint merge l1 l2 :=
+    let fix merge_aux l2 :=
+        match l1, l2 with
+        | [], _ => l2
+        | _, [] => l1
+        | a1::l1', a2::l2' =>
+          if le a1 a2
+          then a1 :: merge l1' l2
+          else a2 :: merge_aux l2'
+        end
+    in merge_aux l2.
+
+  Definition tstack : Type := list (option (list t)).
+
+  (* from Coq stdlib mergesort implementation *)
+  Fixpoint merge_list_to_stack (stack : tstack) (l : list t) : tstack :=
+    match stack with
+    | [] => [Some l]
+    | None :: stack' => Some l :: stack'
+    | Some l' :: stack' => None :: merge_list_to_stack stack' (merge l' l)
+    end.
+
+  (* from Coq stdlib mergesort implementation *)
+  Fixpoint merge_stack (stack : tstack) : list t :=
+    match stack with
+    | [] => []
+    | None :: stack' => merge_stack stack'
+    | Some l :: stack' => merge l (merge_stack stack')
+    end.
+
+  (* from Coq stdlib mergesort implementation *)
+  Fixpoint iter_merge (stack : tstack) (l : list t) : list t :=
+    match l with
+    | [] => merge_stack stack
+    | a::l' => iter_merge (merge_list_to_stack stack [a]) l'
+    end.
+
+  (* from Coq stdlib mergesort implementation *)
+  Definition sort : list t -> list t :=
+    iter_merge [].
+
+  Theorem sort_makes_sorted :
+    forall l l',
+      l' = sort l ->
+      sorted l'.
+  Admitted.
+
+  Theorem sort_permutes :
+    forall l l',
+      l' = sort l ->
+      Permutation l l'.
+  Admitted.
+
+End Sorting.
